Apply the low-level match primitives to the Rewritable type class

Stratego/Stratego.thy
@@ -1,6 +1,6 @@
 section "Stratego"
 theory Stratego
-  imports Main "HOL-Library.Finite_Map"
+  imports Main "HOL-Library.Finite_Map" "HOL-Library.Word"
 begin
 
 no_notation plus (infixl "+" 65)
@@ -24,6 +24,8 @@ class Rewritable =
   fixes match :: "'a \<Rightarrow> 'a \<Rightarrow> ((string, 'a) fmap) option"
   fixes varof :: "'a \<Rightarrow> string option"
   fixes var :: "string \<Rightarrow> 'a"
+  fixes subexprs :: "'a \<Rightarrow> 'a list"
+  fixes map :: "('a \<Rightarrow> 'a) \<Rightarrow> 'a \<Rightarrow> 'a"
   (*assumes "varof (var a) = Some a"
   assumes "traverse f t = traverse f (traverse f t)"*)
 
@@ -50,8 +52,8 @@ abbreviation rewrite_to :: "'a::Rewritable \<Rightarrow> 'a \<Rightarrow> 'a Str
   ("_ \<rightarrow> _") where
   "(s1 \<rightarrow> s2) \<equiv> s1?; s2!"
 
-definition "wheref" :: "('a::Rewritable) Strategy \<Rightarrow> 'a Strategy" where
-  "wheref x = var ''_''?; x; var ''_''!"
+abbreviation "wheref" :: "('a::Rewritable) Strategy \<Rightarrow> 'a Strategy" where
+  "wheref x \<equiv> var ''_''?; x; var ''_''!"
 
 abbreviation conditional_rewrite_to :: "'a::Rewritable \<Rightarrow> 'a \<Rightarrow> 'a Strategy \<Rightarrow> 'a Strategy"
   ("_ \<rightarrow> _ where _") where 
@@ -155,6 +157,20 @@ fun varof_Arithmetic :: "Arithmetic \<Rightarrow> string option" where
 fun var_Arithmetic :: "string \<Rightarrow> Arithmetic" where
   "var_Arithmetic v = Variable v"
 
+fun subexprs_Arithmetic :: "Arithmetic \<Rightarrow> Arithmetic list" where
+  "subexprs_Arithmetic (Add x y) = [x, y]" |
+  "subexprs_Arithmetic (Sub x y) = [x, y]" |
+  "subexprs_Arithmetic (UMinus x) = [x]" |
+  "subexprs_Arithmetic (Number v) = []" |
+  "subexprs_Arithmetic (Variable s) = []"
+
+fun map_Arithmetic where
+  "map_Arithmetic f (Add x y) = (Add (f x) (f y))" |
+  "map_Arithmetic f (Sub x y) = (Sub (f x) (f y))" |
+  "map_Arithmetic f (UMinus x) = (UMinus (f x))" |
+  "map_Arithmetic f (Number v) = (Number v)" |
+  "map_Arithmetic f (Variable s) = (Variable s)"
+
 instance proof qed
 
 (*instance proof
@@ -165,6 +181,8 @@ instance proof qed
     apply (induction t) apply simp sorry
 qed*)
 end
+
+
 
 subsubsection "Rewrite Rules"
 
@@ -240,5 +258,583 @@ text \<open>@{value "eval EvalMinus ((UMinus (Number 10)), fmempty)"}\<close>
 value "eval EvalAdd ((UMinus (Number 10)), fmempty)"
 value "eval EvalAdd ((Add (Number 10) (Number 10)), fmempty)"
 text \<open>@{value "eval EvalAdd ((Add (Number 10) (Number 10)), fmempty)"}\<close>
+
+
+
+
+
+
+class ShallowRewritable =
+  fixes base :: "'a itself \<Rightarrow> Arithmetic itself"
+
+syntax "_type_base" :: "type \<Rightarrow> string" (\<open>(1BASE/(1'(_')))\<close>)
+
+translations "BASE('a)" \<rightharpoonup>
+  "CONST base (CONST Pure.type :: 'a itself)"
+
+print_translation \<open>
+  let
+    fun len_of_itself_tr' ctxt [Const (\<^const_syntax>\<open>Pure.type\<close>, Type (_, [T]))] =
+      Syntax.const \<^syntax_const>\<open>_type_base\<close> $ Syntax_Phases.term_of_typ ctxt T
+  in [(\<^const_syntax>\<open>base\<close>, len_of_itself_tr')] end
+\<close>
+
+(* TODO: can this be automatically generated? *)
+(*datatype ShallowArithmetic =
+  Add string string |
+  Sub string string |
+  UMinus string |
+  Number int
+*)
+
+type_synonym VarName = "string"
+type_synonym Vars = "VarName fset"
+
+type_synonym Scope = "Vars \<times> (VarName \<rightharpoonup> VarName)"
+
+fun remove_var :: "VarName \<Rightarrow> Scope \<Rightarrow> Scope" where
+  "remove_var v (vs, m) = (vs - {|v|}, m)"
+fun add_var :: "VarName \<Rightarrow> Scope \<Rightarrow> Scope" where
+  "add_var v (vs, m) = (vs |\<union>| {|v|}, m)"
+
+
+function fresh_var :: "VarName \<Rightarrow> Scope \<Rightarrow> VarName" where
+  "fresh_var v s = 
+    (if v |\<in>| (fst s) 
+      then fresh_var (v @ ''z'') (remove_var v s)
+      else v)"
+  by fastforce+
+(*(* For some reason, by proving that this function terminates the definition of match_pattern
+   no longer terminates. *)
+termination
+  apply (relation "measure (\<lambda>(v, s). (fcard (fst s)))")
+  apply simp
+  using fcard_fminus1_less by force*)
+
+fun fresh :: "VarName \<Rightarrow> Scope \<Rightarrow> Scope \<times> VarName" where
+  "fresh v s = (let v = fresh_var v s in (add_var v s, v))"
+
+
+lemma fresh [code]:
+  "fresh_var v s = 
+    (if v |\<in>| (fst s) 
+      then fresh_var (v @ ''z'') (remove_var v s)
+      else v)"
+  sorry (* This will not be required when termination is proved *)
+
+
+datatype 'a MATCH =
+  match VarName "'a" |
+  equality VarName VarName (infixl "==" 52) |
+  andthen "'a MATCH" "'a MATCH" (infixl "&&" 50) |
+  condition "'a" |
+  noop
+
+value "subexprs (Add (Add (Number 1) (Number 2)) (Number 3))"
+value "map_MATCH ::Arithmetic MATCH"
+value "case_MATCH ((match ''hey'' (Number 5))::Arithmetic MATCH)"
+value "set_MATCH ((match ''hey'' (Number 5))::Arithmetic MATCH)"
+
+value "map_MATCH (\<lambda>x. ''hi'') ((match ''hey'' (Number 5))::Arithmetic MATCH)"
+
+
+text \<open>The definitions of la and ra help to feed the scope through when generating a match pattern.\<close>
+definition la :: "('b \<Rightarrow> 'a) \<Rightarrow> (Scope \<Rightarrow> Scope \<times> 'b) \<Rightarrow> (Scope \<Rightarrow> Scope \<times> 'a)"
+  (infix "\<langle>" 65)
+  where
+  "la f f' s = (fst (f' s), f (snd (f' s)))"
+
+definition ra :: "(Scope \<Rightarrow> Scope \<times> ('b \<Rightarrow> 'a)) \<Rightarrow> (Scope \<Rightarrow> Scope \<times> 'b) \<Rightarrow> (Scope \<Rightarrow> Scope \<times> 'a)"
+  (infixl "\<rangle>" 54)
+  where
+  "ra f f' s = ((fst (f' (fst (f s)))), (snd (f s)) (snd (f' (fst (f s)))))"
+
+text \<open>Join generates the lhs and feeds the scope through to then generate the rhs.
+      The resulting match pattern is an sequential match of the lhs and rhs, @{term "lhs && rhs"}.
+      The resulting scope is the result of generating the rhs after the lhs.\<close>
+(*definition join :: "('b \<Rightarrow> 'c \<times> ('d::Rewritable) MATCH) \<Rightarrow> ('b \<Rightarrow> 'c \<Rightarrow> 'a \<times> 'd MATCH) \<Rightarrow> 'b \<Rightarrow> 'a \<times> 'd MATCH"
+  (infixl "|>" 53) where
+  "join x y s = 
+    (let (lhs_scope, lhs_match) = x s in
+    (let (rhs_scope, rhs_match) = (y s lhs_scope) in
+    (rhs_scope, (lhs_match && rhs_match))))"
+
+abbreviation descend where
+  "descend f e v \<equiv> (\<lambda>s s'. f e (snd (fresh v s)) s')"*)
+
+fun register_name where
+  "register_name (s, m) vn v = (s, m(vn\<mapsto>v))"
+
+(*
+typedef (overloaded) ('a, 'b) fixed_list =
+  "{l::'b list. LENGTH('a::len) = length l}"
+  by (metis Ex_list_of_length mem_Collect_eq)
+
+lemma "Rep_fixed_list ((Abs_fixed_list [1, 2])::(2, nat) fixed_list) = [1, 2]"
+  sledgehammer
+
+fun convert :: "('a::len, 'b) fixed_list \<Rightarrow> ('a, 'b) fixed_list" where
+  "convert (Abs_fixed_list [x, y]) = (Abs_fixed_list [y, x])"
+*)
+
+(*
+fun chain :: "'b \<Rightarrow> ('a \<Rightarrow> 'b \<Rightarrow> ('b \<times> 'a)) \<Rightarrow> 'a list \<Rightarrow> ('b \<times> 'a list)" where
+  "chain a f [] = (a, [])" |
+  "chain a f (x # xs) =
+    (let (a', x') = f x a in
+    (let (a'', xs') = (chain a' f xs) in (a'', x' # xs')))"
+
+fun replace_subexprs :: "Scope \<Rightarrow> ('a::Rewritable) list \<Rightarrow> Scope \<times> ('a::Rewritable) list" where
+  "replace_subexprs s = chain s (\<lambda>e s'. (let (s'', v) = (fresh ''a'' s') in (s'', var v)))"
+*)
+
+fun replace_subexprs :: "Scope \<Rightarrow> ('a::Rewritable) \<Rightarrow> ('a::Rewritable)" where
+  "replace_subexprs s = map (\<lambda>_. var (snd (fresh ''a'' s)))"
+
+abbreviation generate_subexprs where
+  "generate_subexprs f e s \<equiv> (List.map (\<lambda>e'. snd (f e' (snd (fresh ''a'' s)) s)) (subexprs e))"
+
+fun join :: "('a MATCH) list \<Rightarrow> 'a MATCH" where
+  "join [] = noop" |
+  "join [x] = x" |
+  "join (x # xs) = (x && join xs)"
+
+function match_pattern :: "('a::Rewritable) \<Rightarrow> VarName \<Rightarrow> Scope \<Rightarrow> Scope \<times> 'a MATCH" where
+  "match_pattern e v =
+    (case varof e of
+      Some vn \<Rightarrow> (\<lambda>s. case (snd s) vn of 
+        None \<Rightarrow> (register_name s vn v, noop) |
+        Some v' \<Rightarrow> (register_name s vn v, equality v' v)) |
+      None \<Rightarrow> (\<lambda>s. (s, (match v (replace_subexprs s e) 
+                        && join (generate_subexprs match_pattern e s)))))"
+  using old.prod.exhaust apply blast
+  by fastforce
+
+termination match_pattern sorry
+
+value "match_pattern 
+(Sub (Add (Variable ''x'') (Variable ''y'')) (Variable ''y''))
+''e'' ({|''e''|}, Map.empty)"
+
+(*"match v \<langle> ((\<lambda>y. e) \<langle> fresh ''a'') |> descend match_pattern e ''a'')"
+
+fun match_pattern :: "('a::Rewritable) \<Rightarrow> VarName \<Rightarrow> Scope \<Rightarrow> Scope \<times> 'a MATCH" where
+  "match_pattern (UnaryExpr op e) v =
+    match v \<langle>
+      (UnaryPattern op \<langle> fresh ''a'')
+    |> descend match_pattern e ''a''" |
+  "match_pattern (BinaryExpr op e1 e2) v =
+    match v \<langle> 
+      (BinaryPattern op \<langle> fresh ''a'' \<rangle> fresh ''b'')
+    |> descend match_pattern e1 ''a''
+    |> descend match_pattern e2 ''b''" |
+  "match_pattern (ConditionalExpr b e1 e2) v =
+    match v \<langle>
+      (ConditionalPattern \<langle> fresh ''a'' \<rangle> fresh ''b'' \<rangle> fresh ''c'')
+    |> descend match_pattern b ''a''
+    |> descend match_pattern e1 ''b''
+    |> descend match_pattern e2 ''c''" |
+  \<comment> \<open>If a variable is reused, generate an equality check, else, generate a noop.\<close>
+  "match_pattern (VariableExpr vn st) v = 
+    (\<lambda>s. case (snd s) vn of 
+      None \<Rightarrow> (register_name s vn v, noop) |
+      Some v' \<Rightarrow> (register_name s vn v, equality v' v))" |
+  "match_pattern (ConstantExpr c) v =
+    (\<lambda>s. (s, match v (ConstantPattern c)))" |
+  "match_pattern (ConstantVar c) v =
+    (\<lambda>s. (s, match v (ConstantVarPattern c)))" |
+  "match_pattern _ v = (\<lambda>s. (s, noop))"*)
+
+definition gen_pattern :: "('a::Rewritable) \<Rightarrow> VarName \<Rightarrow> 'a MATCH" where
+  "gen_pattern p v = snd (match_pattern p v ({|v|}, Map.empty))"
+
+subsubsection \<open>Match Primitive Semantics\<close>
+type_synonym 'a Subst = "VarName \<rightharpoonup> 'a::Rewritable"
+
+fun equal_ignore_vars :: "'a::Rewritable \<Rightarrow> 'a \<Rightarrow> bool" where
+  "equal_ignore_vars e1 e2 = ((map (\<lambda>_. var ''a'') e1) = (map (\<lambda>_. var ''a'') e2))"
+
+fun eval_match :: "('a::Rewritable) MATCH \<Rightarrow> 'a Subst \<Rightarrow> ('a Subst) option" where
+  "eval_match (match v e) s =
+    (case s v of
+      Some e' \<Rightarrow>
+        (if equal_ignore_vars e e' then
+          Some (s((List.map (the o varof) (subexprs e)) [\<mapsto>] subexprs e')) else None) |
+      None \<Rightarrow> None)" |
+  "eval_match (equality v1 v2) s =
+    (if v1 \<in> dom s \<and> v2 \<in> dom s \<and> s v1 = s v2 then Some s else None)" |
+  "eval_match (andthen m1 m2) s =
+      (case eval_match m1 s of 
+        None \<Rightarrow> None |
+        Some s' \<Rightarrow> eval_match m2 s')" |
+  "eval_match noop s = Some s" |
+  "eval_match (condition sc) s = None"
+
+(*
+fun eval_match :: "'a MATCH \<Rightarrow> 'a Subst \<Rightarrow> ('a Subst) option" where
+  "eval_match (match v (UnaryPattern op1 x)) s =
+    (case s v of 
+      Some (UnaryExpr op2 xe) \<Rightarrow>
+        (if op1 = op2 then
+          (if x \<in> dom s then
+            (if s x = Some xe then Some s else None)
+          else Some (s(x\<mapsto>xe)))
+         else None) |
+      Some _ \<Rightarrow> None |
+      None \<Rightarrow> None)" |
+  "eval_match (match v (BinaryPattern op1 x y)) s =
+    (case s v of
+      Some (BinaryExpr op2 xe ye) \<Rightarrow>
+        (if op1 = op2 
+          then 
+          (if x \<in> dom s \<and> s x \<noteq> Some xe then None else 
+          (if y \<in> dom s \<and> s y \<noteq> Some ye then None else 
+          (if x \<in> dom s \<and> y \<in> dom s then Some s else
+          (if x \<in> dom s then Some (s(y\<mapsto>ye)) else
+          (if y \<in> dom s then Some (s(x\<mapsto>xe)) else
+          Some (s(x\<mapsto>xe, y\<mapsto>ye)))))))
+          else None) |
+      Some _ \<Rightarrow> None |
+      None \<Rightarrow> None)" |
+  "eval_match (match v (ConditionalPattern c tb fb)) s =
+    (case s v of
+      Some (ConditionalExpr ce te fe) \<Rightarrow>
+        (if c \<in> dom s \<and> s c \<noteq> Some ce then None else 
+          (if tb \<in> dom s \<and> s tb \<noteq> Some te then None else
+          (if fb \<in> dom s \<and> s fb \<noteq> Some fe then None else 
+          (if c \<in> dom s \<and> tb \<in> dom s \<and> fb \<in> dom s then Some s else
+          (if c \<in> dom s \<and> tb \<in> dom s then Some (s(fb\<mapsto>fe)) else
+          (if c \<in> dom s \<and> fb \<in> dom s then Some (s(tb\<mapsto>te)) else
+          (if tb \<in> dom s \<and> fb \<in> dom s then Some (s(c\<mapsto>ce)) else
+          (if c \<in> dom s then Some (s(tb\<mapsto>te, fb\<mapsto>fe)) else
+          (if tb \<in> dom s then Some (s(c\<mapsto>ce, fb\<mapsto>fe)) else
+          (if fb \<in> dom s then Some (s(c\<mapsto>ce, tb\<mapsto>te)) else
+          Some (s(c\<mapsto>ce, tb\<mapsto>te, fb\<mapsto>fe)))))))))))) |
+      Some _ \<Rightarrow> None |
+      None \<Rightarrow> None)" |
+  "eval_match (match v (ConstantPattern c1)) s =
+    (case s v of 
+      Some (ConstantExpr c2) \<Rightarrow>
+        (if c1 = c2 then Some s else None) |
+      Some _ \<Rightarrow> None |
+      None \<Rightarrow> None)" |
+  "eval_match (equality v1 v2) s =
+    (if v1 \<in> dom s \<and> v2 \<in> dom s \<and> s v1 = s v2 then Some s else None)" |
+  "eval_match (andthen m1 m2) s =
+      (case eval_match m1 s of 
+        None \<Rightarrow> None |
+        Some s' \<Rightarrow> eval_match m2 s')" |
+  "eval_match noop s = Some s" |
+  "eval_match (condition sc) s = (if eval_condition sc then Some s else None)" |
+  "eval_match _ s = None"
+*)
+
+
+subsection \<open>Combining Rules\<close>
+
+datatype 'a Rules =
+  base "'a::Rewritable" |
+  cond "'a MATCH" "'a Rules" (infixl "?" 52) |
+  else "'a Rules" "'a Rules" (infixl "else" 50) |
+  seq "'a Rules" "'a Rules" (infixl "\<then>" 49) |
+  choice "('a Rules) list"
+
+function ground_expr :: "'a::Rewritable \<Rightarrow> Scope \<Rightarrow> 'a" where
+  "ground_expr e (s, m) =
+    (case varof e of
+      Some v \<Rightarrow>(case m v of None \<Rightarrow> var v 
+                | Some v' \<Rightarrow> var v') |
+      None \<Rightarrow> map (\<lambda>e'. ground_expr e' (s, m)) e)"
+  apply auto[1]
+  by fastforce
+
+termination ground_expr sorry
+(*
+    UnaryExpr op (ground_expr e s)" |
+  "ground_expr (BinaryExpr op e1 e2) s = 
+    BinaryExpr op (ground_expr e1 s) (ground_expr e2 s)" |
+  "ground_expr (ConditionalExpr b e1 e2) s = 
+    ConditionalExpr (ground_expr b s) (ground_expr e1 s) (ground_expr e2 s)" |
+  "ground_expr (VariableExpr vn st) (s, m) = 
+    (case m vn of None \<Rightarrow> VariableExpr vn st 
+                | Some v' \<Rightarrow> VariableExpr v' st)" |
+  "ground_expr e s = e"*)
+
+(*fun ground_result :: "Result \<Rightarrow> Scope \<Rightarrow> Result" where
+  "ground_result (ExpressionResult e) s = ExpressionResult (ground_expr e s)" |
+  "ground_result (forZero e) s = forZero (ground_expr e s)"
+
+fun ground_condition :: "SideCondition \<Rightarrow> Scope \<Rightarrow> SideCondition" where
+  "ground_condition (IsConstantExpr p) s = (IsConstantExpr (ground_expr p s))" |
+  "ground_condition (IsIntegerStamp p) s = (IsIntegerStamp (ground_expr p s))" |
+  "ground_condition (IsBoolStamp p) s = (IsBoolStamp (ground_expr p s))" |
+  "ground_condition (WellFormed st) s = (WellFormed st)" |
+  "ground_condition (IsStamp e st) s = (IsStamp (ground_expr e s) st)" |
+  "ground_condition (IsConstantValue e s' v) s = (IsConstantValue (ground_expr e s) (ground_expr s' s) v)" |
+  "ground_condition (AlwaysDistinct e1 e2) s = (AlwaysDistinct (ground_expr e1 s) (ground_expr e2 s))" |
+  "ground_condition (NeverDistinct e1 e2) s = (NeverDistinct (ground_expr e1 s) (ground_expr e2 s))" |  
+  "ground_condition (StampUnder e1 e2) s = (StampUnder (ground_expr e1 s) (ground_expr e2 s))" |
+  "ground_condition (UpMaskEquals e m) s = (UpMaskEquals (ground_expr e s) m)" |
+  "ground_condition (DownMaskEquals e m) s = (DownMaskEquals (ground_expr e s) m)" |
+  "ground_condition (UpMaskCancels e1 e2) s = (UpMaskCancels (ground_expr e1 s) (ground_expr e2 s))" |
+  "ground_condition (PowerOf2 e) s = (PowerOf2 (ground_expr e s))" |
+  "ground_condition (IsBool e) s = (IsBool (ground_expr e s))" |
+  "ground_condition (And sc1 sc2) s = And (ground_condition sc1 s) (ground_condition sc2 s)" |
+  "ground_condition (Not sc) s = Not (ground_condition sc s)" |
+  "ground_condition (Empty) s = Empty"*)
+
+fun generate :: "'a::Rewritable \<Rightarrow> 'a \<Rightarrow> 'a \<Rightarrow> 'a Rules" where
+  "generate p r sc = 
+    (let (s, m) = match_pattern p ''e'' ({||}, (\<lambda>x. None))
+     in ((m && condition (ground_expr sc s)) ? (base (ground_expr r s))))"
+
+subsubsection \<open>Rules Semantics\<close>
+definition start_unification where
+  "start_unification e = ((\<lambda>x. None)(STR ''e'' := Some e))"
+
+text \<open>Replace any variable expressions with value in a substitution.\<close>
+fun evaluated_terms where
+  "evaluated_terms f es s = (List.map (\<lambda>e. f e s) es)"
+
+fun has_none :: "('a option) list \<Rightarrow> bool" where
+  "has_none [] = False" |
+  "has_none (x # xs) = ((x = None) \<and> has_none xs)"
+
+function eval_expr :: "'a::Rewritable \<Rightarrow> 'a Subst \<Rightarrow> 'a option" where
+  "eval_expr e u =
+    (case varof e of
+        Some v \<Rightarrow> u v
+      | None \<Rightarrow> 
+        (if has_none (evaluated_terms eval_expr (subexprs e) u)
+          then None
+          else Some (map (the o (\<lambda>e'. eval_expr e' u)) e)))"
+  by fastforce+
+
+termination eval_expr sorry
+
+(*
+  "eval_expr (UnaryExpr op e) u = (case (eval_expr e u)
+    of None \<Rightarrow> None | Some e' \<Rightarrow> Some (UnaryExpr op e'))" |
+  "eval_expr (BinaryExpr op e1 e2) u = (case (eval_expr e1 u)
+    of None \<Rightarrow> None | Some e1' \<Rightarrow> 
+    (case (eval_expr e2 u)
+      of None \<Rightarrow> None | Some e2' \<Rightarrow> Some (BinaryExpr op e1' e2')))" |
+  "eval_expr (ConditionalExpr e1 e2 e3) u = (case (eval_expr e1 u)
+    of None \<Rightarrow> None | Some e1' \<Rightarrow>
+    (case (eval_expr e2 u)
+      of None \<Rightarrow> None | Some e2' \<Rightarrow>
+        (case (eval_expr e2 u)
+          of None \<Rightarrow> None | Some e3' \<Rightarrow> Some (ConditionalExpr e1' e2' e3'))))" |
+  "eval_expr e u = Some e"
+
+
+fun eval_result :: "Result \<Rightarrow> Subst \<Rightarrow> IRExpr option" where
+  "eval_result (ExpressionResult e) s = (eval_expr e s)" |
+  "eval_result (forZero e) s = (case eval_expr e s of
+    None \<Rightarrow> None |
+    Some r \<Rightarrow> Some (ConstantExpr (IntVal (stp_bits (stamp_expr r)) 0)))"
+
+lemma remove1_size:
+  "x \<in> set xs \<Longrightarrow> size (remove1 x xs) < size xs"
+  by (metis diff_less length_pos_if_in_set length_remove1 zero_less_one)
+*)
+
+inductive eval_rules :: "('a::Rewritable) Rules \<Rightarrow> 'a Subst \<Rightarrow> 'a option \<Rightarrow> bool" where
+  \<comment> \<open>Evaluate the result\<close>
+  "eval_rules (base e) u (eval_expr e u)" |
+
+  \<comment> \<open>Evaluate a condition\<close>
+  "\<lbrakk>eval_match m u = Some u' \<and>
+    eval_rules r u' e\<rbrakk>
+   \<Longrightarrow> eval_rules (cond m r) u e" |
+  "\<lbrakk>eval_match m u = None\<rbrakk>
+   \<Longrightarrow> eval_rules (cond m r) u None" |
+
+  \<comment> \<open>Evaluate else\<close>
+  "\<lbrakk>eval_rules r1 u (Some r)\<rbrakk>
+   \<Longrightarrow> eval_rules (r1 else r2) u (Some r)" |
+  "\<lbrakk>eval_rules r1 u None \<and>
+    eval_rules r2 u e\<rbrakk>
+   \<Longrightarrow> eval_rules (r1 else r2) u e" |
+
+  \<comment> \<open>Evaluate choice\<close>
+  "\<lbrakk>rule \<in> set rules \<and>
+    eval_rules rule u (Some r)\<rbrakk>
+   \<Longrightarrow> eval_rules (choice rules) u (Some r)" |
+  "\<lbrakk>\<forall> rule \<in> set rules. eval_rules rule u None\<rbrakk>
+   \<Longrightarrow> eval_rules (choice rules) u None" |
+  "\<lbrakk>rules = []\<rbrakk>
+   \<Longrightarrow> eval_rules (choice rules) u None" |
+
+  \<comment> \<open>Evaluate sequential\<close>
+  "\<lbrakk>eval_rules r1 u (Some e') \<and>
+    eval_rules r2 (u(''e'' \<mapsto> e')) r\<rbrakk>
+   \<Longrightarrow> eval_rules (r1 \<then> r2) u r" |
+  "\<lbrakk>eval_rules r1 u None \<and>
+    eval_rules r2 u r\<rbrakk>
+   \<Longrightarrow> eval_rules (r1 \<then> r2) u r"
+
+
+
+
+
+
+
+
+
+
+
+subsection \<open>Rule Optimization\<close>
+
+fun elim_noop :: "'a MATCH \<Rightarrow> 'a MATCH" where
+  "elim_noop (lhs && noop) = elim_noop lhs" |
+  "elim_noop (noop && rhs) = elim_noop rhs" |
+  "elim_noop (lhs && rhs) = ((elim_noop lhs) && (elim_noop rhs))" |
+  "elim_noop m = m"
+
+fun eliminate_noop :: "'a::Rewritable Rules \<Rightarrow> 'a Rules" where
+  "eliminate_noop (base e) = base e" |
+  "eliminate_noop (m ? r) = elim_noop m ? eliminate_noop r" |
+  "eliminate_noop (r1 else r2) = (eliminate_noop r1 else eliminate_noop r2)" |
+  "eliminate_noop (choice rules) = choice (List.map eliminate_noop rules)" |
+  "eliminate_noop (r1 \<then> r2) = (eliminate_noop r1 \<then> eliminate_noop r2)"
+
+fun elim_empty :: "'a MATCH \<Rightarrow> 'a MATCH" where
+  "elim_empty (condition Empty) = noop" |
+  "elim_empty (m1 && m2) = (elim_empty m1 && elim_empty m2)" |
+  "elim_empty m = m"
+
+fun eliminate_empty :: "'a::Rewritable Rules \<Rightarrow> 'a Rules" where
+  "eliminate_empty (base e) = base e" |
+  "eliminate_empty (m ? r) = elim_empty m ? eliminate_empty r" |
+  "eliminate_empty (r1 else r2) = (eliminate_empty r1 else eliminate_empty r2)" |
+  "eliminate_empty (choice rules) = choice (List.map eliminate_empty rules)" |
+  "eliminate_empty (r1 \<then> r2) = (eliminate_empty r1 \<then> eliminate_empty r2)"
+
+
+notation plus (infixl "+" 65)
+fun combined_size :: "'a::Rewritable Rules \<Rightarrow> nat" where
+  "combined_size (m ? r) = (2 * size m) + combined_size r" |
+  "combined_size (base e) = 0" |
+  "combined_size (r1 else r2) = combined_size r1 + combined_size r2" |
+  "combined_size (choice (rule # rules)) = 1 + combined_size rule + combined_size (choice rules)" |
+  "combined_size (choice []) = 1" |
+  "combined_size (r1 \<then> r2) = combined_size r1 + combined_size r2"
+no_notation plus (infixl "+" 65)
+
+function (sequential) lift_match :: "'a::Rewritable Rules \<Rightarrow> 'a Rules" where
+  "lift_match (r1 else r2) = ((lift_match r1) else (lift_match r2))" |
+  "lift_match (choice rules) = choice (List.map lift_match rules)" |
+  "lift_match ((m1 && m2) ? r) = (lift_match (m1 ? (m2 ? r)))" |
+  "lift_match (m ? r) = m ? (lift_match r)" |
+  "lift_match (base e) = (base e)" |
+  "lift_match (r1 \<then> r2) = (lift_match r1 \<then> lift_match r2)"
+  by pat_completeness auto
+termination lift_match
+  apply (relation "measures [combined_size, size]") apply auto[1]
+  apply auto[1] apply auto[1] apply simp
+  subgoal for rules x apply (induction rules) apply simp by fastforce
+  apply simp subgoal for m2 r apply (cases m2) sorry
+        apply simp+
+  apply blast
+  by auto
+
+fun join_conditions :: "'a::Rewritable Rules \<Rightarrow> 'a Rules option" where
+  "join_conditions (m1 ? r1 else m2 ? r2) = 
+    (if m1 = m2
+      then Some (m1 ? (r1 else r2)) else None)" |
+  "join_conditions (m1 ? (m2 ? r1)) = 
+    (if m1 = m2
+      then Some ((m1 ? r1)) else None)" |
+  "join_conditions r = None"
+
+function lift_common :: "'a::Rewritable Rules \<Rightarrow> 'a Rules" where
+  "lift_common (r1 else r2) = (
+    case join_conditions (r1 else r2) 
+    of Some r \<Rightarrow> lift_common r |
+       None \<Rightarrow> (lift_common r1 else lift_common r2))" |
+  "lift_common (m ? r) = (
+    case join_conditions (m ? r) 
+    of Some r' \<Rightarrow> lift_common r' |
+       None \<Rightarrow> (m ? lift_common r))" |
+  "lift_common (choice rules) = choice (List.map lift_common rules)" |
+  "lift_common (base e) = base e" |
+  "lift_common (r1 \<then> r2) = (lift_common r1 \<then> lift_common r2)"
+  using combined_size.cases 
+  apply (smt (verit, ccfv_threshold))
+  by simp+
+termination
+  apply (relation "measures [size]") apply auto[1]
+    apply simp subgoal for r1 r2 apply (induction r1 rule: join_conditions.induct) by simp+
+   apply auto[1] sorry
+
+notation plus (infixl "+" 65)
+fun common_size :: "'a::Rewritable Rules \<Rightarrow> nat" where
+  "common_size (m ? r) = 1 + common_size r" |
+  "common_size (base e) = 0" |
+  "common_size (r1 else r2) = 1 + common_size r1 + common_size r2" |
+  "common_size (choice (rule # rules)) = 1 + common_size rule + common_size (choice rules)" |
+  "common_size (choice []) = 0" |
+  "common_size (r1 \<then> r2) = 1 + common_size r1 + common_size r2"
+no_notation plus (infixl "+" 65)
+
+fun find_common :: "'a::Rewritable MATCH \<Rightarrow> 'a Rules \<Rightarrow> 'a Rules option" where
+  "find_common m (m' ? r) = (if m = m' then Some r else None)" |
+  "find_common m r = None"
+
+fun find_uncommon :: "'a::Rewritable MATCH \<Rightarrow> 'a Rules \<Rightarrow> 'a Rules option" where
+  "find_uncommon m (m' ? r) = (if m = m' then None else Some (m' ? r))" |
+  "find_uncommon m r = Some r"
+
+definition join_common :: "'a::Rewritable MATCH \<Rightarrow> 'a Rules list \<Rightarrow> 'a Rules list" where
+  "join_common m rules = List.map_filter (find_common m) rules"
+
+definition join_uncommon :: "'a::Rewritable MATCH \<Rightarrow> 'a Rules list \<Rightarrow> 'a Rules list" where
+  "join_uncommon m rules = List.map_filter (find_uncommon m) rules"
+
+function (sequential) combine_conditions :: "'a::Rewritable Rules \<Rightarrow> 'a Rules" where
+  "combine_conditions (base e) = base e" |
+  "combine_conditions (r1 else r2) = (combine_conditions r1 else combine_conditions r2)" |
+  "combine_conditions (m ? r) = (m ? combine_conditions r)" |
+  "combine_conditions (choice ((m ? r) # rules)) = 
+    choice ((m ? combine_conditions (choice (r # join_common m rules)))
+      # [combine_conditions (choice (join_uncommon m rules))])" |
+  "combine_conditions (choice rules) = 
+    choice (List.map combine_conditions rules)" |
+  "combine_conditions (r1 \<then> r2) = (combine_conditions r1 \<then> combine_conditions r2)"
+  apply pat_completeness+
+  by simp+
+
+termination combine_conditions sorry
+
+fun eliminate_choice :: "'a::Rewritable Rules \<Rightarrow> 'a Rules" where
+  "eliminate_choice (base e) = base e" |
+  "eliminate_choice (r1 else r2) = (eliminate_choice r1 else eliminate_choice r2)" |
+  "eliminate_choice (m ? r) = (m ? eliminate_choice r)" |
+  "eliminate_choice (choice (r # [])) = eliminate_choice r" |
+  "eliminate_choice (choice rules) = 
+    choice (List.map eliminate_choice rules)" |
+  "eliminate_choice (r1 \<then> r2) = (eliminate_choice r1 \<then> eliminate_choice r2)"
+
+definition optimized_export where
+  "optimized_export = eliminate_choice \<circ> combine_conditions o lift_common o lift_match o eliminate_noop o eliminate_empty"
+
+
+value "optimized_export
+(generate
+(Add (Sub (Variable ''x'') (Variable ''y'')) (Variable ''y''))
+(Variable ''x'')
+(Variable ''y''))"
+
+
+fun compile :: "'a::Rewritable Strategy \<Rightarrow> 'a Rules" where
+  "compile (s1 \<rightarrow> s2) = gen_pattern s1 ''e'' ? base s2"(* |
+  "compile (s1 \<rightarrow> s2 where c) = ((gen_pattern s1 ''e'') ? base s2)"*)
+
+value "compile RedundantAdd"
+value "compile RedundantSub"
+value "compile ShiftConstRight"
+value "compile EvalMinus1"
+value "compile EvalAdd"
 
 end
